WIP

HumanEvalLean/HumanEval1.lean
@@ -1,7 +1,152 @@
 module
 
-def separate_paren_groups : Unit :=
-  ()
+import Std.Tactic.Do
+
+def separateParenGroups (parenString : String) : Array String := Id.run do
+  let mut result := #[]
+  let mut curr := ""
+  let mut depth := 0
+  for c in parenString do
+    if c == '(' then
+      depth := depth + 1
+      curr := curr.push c
+    else if c == ')' then
+      depth := depth - 1
+      curr := curr.push c
+      if depth = 0 then
+        result := result.push curr
+        curr := ""
+  return result
+
+section Verification
+
+inductive Paren where
+  | open : Paren
+  | close : Paren
+
+inductive IsBalanced : List Paren → Prop where
+  | empty : IsBalanced []
+  | append : IsBalanced l₁ → IsBalanced l₂ → IsBalanced (l₁ ++ l₂)
+  | enclose : IsBalanced l → IsBalanced (.open :: l ++ [.close])
+
+inductive IsGroup : List Paren → Prop where
+  | enclose : IsBalanced l → IsGroup (.open :: l ++ [.close])
+
+def parens (s : String) : List Paren :=
+  s.toList.filterMap (fun c => if c = '(' then some .open else if c = ')' then some .close else none)
+
+/-
+@[spec]
+theorem Spec.forIn_list
+    {xs : List α} {init : β} {f : α → β → m (ForInStep β)}
+    (inv : Invariant xs β ps)
+    (step : ∀ pref cur suff (h : xs = pref ++ cur :: suff) b,
+      Triple
+        (f cur b)
+        (inv.1 (⟨pref, cur::suff, h.symm⟩, b))
+        (fun r => match r with
+          | .yield b' => inv.1 (⟨pref ++ [cur], suff, by simp [h]⟩, b')
+          | .done b' => inv.1 (⟨xs, [], by simp⟩, b'), inv.2)) :
+    Triple (forIn xs init f) (inv.1 (⟨[], xs, rfl⟩, init)) (fun b => inv.1 (⟨xs, [], by simp⟩, b), inv.2) := by
+  simp only [← forIn'_eq_forIn]
+  exact Spec.forIn'_list inv step
+-/
+
+namespace Std.Do
+variable {β : Type u} {m : Type u → Type v} {ps : PostShape.{u}}
+variable [Monad m] [WPMonad m ps]
+
+@[spec]
+theorem Spec.forIn_string
+    {s : String} {init : β} {f : Char → β → m (ForInStep β)}
+    (inv : PostCond (s.Pos × β) ps)
+    (step : ∀ pos b (h : pos ≠ s.endPos),
+      Triple
+        (f (pos.get h) b)
+        (inv.1 (pos, b))
+        (fun r => match r with
+          | .yield b' => inv.1 (pos.next h, b')
+          | .done b' => inv.1 (s.endPos, b'), inv.2)) :
+    Triple (forIn s init f) (inv.1 (s.startPos, init)) (fun b => inv.1 (s.endPos, b), inv.2) := sorry
+
+end Std.Do
+
+open Std.Do
+
+/-- You might want to invoke `Pos.Splits.exists_eq_singleton_append` to be able to apply this. -/
+theorem String.Pos.Splits.of_next {s : String} {p : s.Pos} {h}
+    (h : (p.next h).Splits (t₁ ++ singleton c) t₂) : p.Splits t₁ (singleton c ++ t₂) := by
+  sorry
+  --   -- (h : p.Splits t₁ (singleton c ++ t₂)) : (p.next h.ne_endPos_of_singleton).Splits (t₁ ++ singleton c) t₂
+  --   := by
+  -- generalize h.ne_endPos_of_singleton = hp
+  -- obtain ⟨rfl, rfl, rfl⟩ := by simpa using h.eq (splits_next_right p hp)
+  -- exact splits_next p hp
+
+@[simp]
+theorem List.self_eq_filter {l : List α} {p : α → Bool} : l = l.filter p ↔ ∀ a ∈ l, p a := by
+  simp [eq_comm (a := l)]
+
+theorem goal₁ {s : String} {h : IsBalanced (parens s)} :
+    (separateParenGroups s).toList.flatMap String.toList = s.toList.filter (fun c => c = '(' ∨ c = ')') := by
+  generalize hwp : separateParenGroups s = w
+  apply Std.Do.Id.of_wp_run_eq hwp
+  mvcgen
+  case vc1.inv => exact ⇓⟨pos, ⟨curr, depth, result⟩⟩ =>
+    ⌜(curr = "" ↔ depth = 0) ∧ ∀ t₁ t₂, pos.Splits t₁ t₂ → result.toList.flatMap String.toList ++ curr.toList = t₁.toList.filter (fun c => c = '(' ∨ c = ')')⌝
+  next pos _ h curr _ depth result h₁ ih =>
+    simp at ih
+    simp
+    intro t₁ t₂ hsp
+    obtain ⟨t₁, rfl⟩ := hsp.exists_eq_append_singleton
+    rw [← List.append_assoc, ih.2 _ _ hsp.of_next]
+    simp only [↓Char.isValue, beq_iff_eq] at h₁
+    simp [h₁]
+  next pos _ h curr _ depth result h₁ h₂ decreasedDepth newCurr newDepth ih =>
+    simp at ih
+    simp [newCurr]
+    intro t₁ t₂ hsp
+    obtain ⟨t₁, rfl⟩ := hsp.exists_eq_append_singleton
+    rw [← List.append_assoc, ih _ _ hsp.of_next]
+    simp at h₂
+    simp [h₂]
+  next pos _ h curr _ depth result h₁ h₂ decreasedDepth newCurr hd ih =>
+    simp at ih
+    simp [newCurr]
+    intro t₁ t₂ hsp
+    obtain ⟨t₁, rfl⟩ := hsp.exists_eq_append_singleton
+    rw [← List.append_assoc, ih _ _ hsp.of_next]
+    simp at h₂
+    simp [h₂]
+  next pos _ h curr _ depth h₁ h₂ ih =>
+    simp at ih
+    simp
+    intro t₁ t₂ hsp
+    obtain ⟨t₁, rfl⟩ := hsp.exists_eq_append_singleton
+    rw [ih _ _ hsp.of_next]
+    simp at h₁ h₂
+    simp [h₁, h₂]
+  next => simp
+  next ih =>
+    simp at ih
+    simp [← ih]
+
+
+
+
+
+
+
+
+
+
+
+
+
+theorem goal₂ {s : String} {h : IsBalanced (parens s)} :
+    ∀ t ∈ separateParenGroups s, IsGroup (parens t) := sorry
+
+end Verification
 
 /-!
 ## Prompt
